Update Proof System

CPL_Proof_System.thy
@@ -1,6 +1,92 @@
 theory "CPL_Proof_System"
-  imports Main "CPL_Instance" "CPL_Utils"
+  imports Main "CPL_Syntax" "CPL_Semantic"
 begin
+
+(* ================= Auxiliary Functions ================= *)
+
+(* Note: Explain why we use nat <the cardinality of keys> here. The function can't work with set constructors*)
+function allMaps :: "Variable set \<Rightarrow> 'a set \<Rightarrow> 'a Valuation set" where
+"allMaps keys values = (if ((card keys) > 0)
+  then (
+    let
+      k = (SOME x. x \<in> keys);
+      reduced_keys = (keys - {k})
+    in (
+      {
+        m(k \<mapsto> v) | m v. v \<in> values \<and> m \<in> (allMaps reduced_keys values)
+      }
+    )
+  )
+  else { Map.empty }
+)"
+  by auto
+
+fun HOmap :: "'a Valuation \<Rightarrow> Variable list \<Rightarrow> 'a list" where
+"HOmap f var_list = (if ((set var_list) \<subseteq> (dom f))
+  then [the (f v). v \<leftarrow> var_list]
+  else []
+)"
+
+(* Note: |` is called restrict_map operator. m |` A = (\<lambda>x. if x \<in> A then m x else None) *)
+fun projectValuation :: "'a Valuation \<Rightarrow> Variable set \<Rightarrow> 'a Valuation" where
+"projectValuation f V = (if (V \<subseteq> (dom f))
+  then f |` V
+  else Map.empty
+)"
+
+fun buildValuation :: "Variable list \<Rightarrow> 'a list \<Rightarrow> 'a Valuation"  where
+"buildValuation [] [] = Map.empty " |
+"buildValuation variables values = (if (length(variables) = length(values))
+  then Map.empty (variables [\<mapsto>] values)
+  else Map.empty
+)"
+
+fun isParent :: "'a Judgement \<Rightarrow> 'a Judgement \<Rightarrow> Formula \<Rightarrow> bool" where
+"isParent \<J>\<^sub>1 \<J>\<^sub>2 \<phi> = (
+  let
+    formula_list = (formulaToList \<phi>);
+    \<psi>\<^sub>1 = (FoI (Index \<J>\<^sub>1) formula_list);
+    \<psi>\<^sub>2 = (FoI (Index \<J>\<^sub>2) formula_list)
+  in ( case (\<psi>\<^sub>1) of
+    (Atom r var_list) \<Rightarrow> False |
+    (Forall x \<phi>\<^sub>1) \<Rightarrow> (
+      ( (Index \<J>\<^sub>1) = (Index \<J>\<^sub>2) - 1 ) \<and>
+      (\<psi>\<^sub>2 = \<phi>\<^sub>1)
+    ) |
+    (Exists x \<phi>\<^sub>1) \<Rightarrow> (
+      ((Index \<J>\<^sub>1) = (Index \<J>\<^sub>2) - 1 ) \<and>
+      (\<psi>\<^sub>2 = \<phi>\<^sub>1)
+    ) |
+    (And \<phi>\<^sub>1 \<phi>\<^sub>2) \<Rightarrow> (
+      (
+        ( (Index \<J>\<^sub>1) = (Index \<J>\<^sub>2) - 1 ) \<and>
+        (\<psi>\<^sub>2 = \<phi>\<^sub>1)
+      ) \<or> (
+        ( (Index \<J>\<^sub>1) = (Index \<J>\<^sub>2) - 2 ) \<and>
+        (\<psi>\<^sub>2 = \<phi>\<^sub>2)
+      )
+    )
+  )
+)"
+
+function existSq :: "Variable set \<Rightarrow> Formula \<Rightarrow> Formula" where
+"existSq vars \<phi> = (if ((card vars) > 0)
+  then (
+    let
+      v = (SOME x. x\<in> vars);
+      reduced_vars = (vars - {v})
+    in (
+      Exists v (existSq reduced_vars \<phi>)
+    )
+  )
+  else \<phi>
+)"
+  by auto
+
+termination existSq
+  apply (relation "measures [\<lambda>(vars, \<phi>). card vars]")
+  apply(auto)
+  by (simp add: card_gt_0_iff some_in_eq)
 
 (* ================= Proof System Functions ================= *)
 
@@ -8,14 +94,14 @@ fun isAtom :: "'a Judgement \<Rightarrow> Formula \<Rightarrow> 'a Structure \<R
 "isAtom \<J> \<phi> \<B> = (
   let
     \<psi> = (FoI (Index \<J>) (formulaToList \<phi>));
-    interpretation = (Interp \<B>)
+    \<I> = (Interp \<B>)
   in
     (isFormulaAtom \<psi>) \<and>
-    ((Vars \<J>) = (set (VarList \<psi>))) \<and>
-    (case (interpretation (Rel \<psi>)) of
+    ((Vars \<J>) = (set (atom_vars \<psi>))) \<and>
+    (case (\<I> (atom_rel \<psi>)) of
       None \<Rightarrow> False |
       Some set_of_list \<Rightarrow> (
-        (Funcs \<J>) = { buildValuation (VarList \<psi>) l | l. l \<in> set_of_list }
+        (Funcs \<J>) = { buildValuation (atom_vars \<psi>) l | l. l \<in> set_of_list }
       )
     )
 )"
@@ -43,11 +129,9 @@ fun isDualProjection :: "'a Judgement \<Rightarrow> 'a Judgement \<Rightarrow> F
       ( y \<in> (Vars \<J>\<^sub>2) )  \<and>
       ( (Vars \<J>\<^sub>1) = (Vars \<J>\<^sub>2) - ({y}) )  \<and>
       (
-        {
-          h \<in> (allMaps (card (Vars \<J>\<^sub>1)) (Vars \<J>\<^sub>1) (Univ \<B>)). (
-            \<forall>b \<in> (Univ \<B>). h(y \<mapsto> b) \<in> (Funcs \<J>\<^sub>2)
-          )
-        } = (Funcs \<J>\<^sub>1)
+        (Funcs \<J>\<^sub>1) = {
+          h \<in> (allMaps (Vars \<J>\<^sub>1) (Univ \<B>)). ( \<forall>b \<in> (Univ \<B>). h(y \<mapsto> b) \<in> (Funcs \<J>\<^sub>2))
+        }
       )
     )
   )
@@ -61,14 +145,15 @@ fun isJoin :: "'a Judgement \<Rightarrow> 'a Judgement \<Rightarrow> 'a Judgemen
   ( (isParent \<J> \<J>\<^sub>1 \<phi>) \<and> (isParent \<J> \<J>\<^sub>2 \<phi>) ) \<and>
   (
     let
-      variables = (Vars \<J>\<^sub>1) \<union> (Vars \<J>\<^sub>2)
+      variables = (Vars \<J>\<^sub>1) \<union> (Vars \<J>\<^sub>2);
+      valuations = (allMaps variables (Univ \<B>))
     in (
-      {
-        f \<in> (allMaps (card variables) variables (Univ \<B>)). (
+      (Funcs \<J>) = {
+        f \<in> valuations. (
           ( (projectValuation f (Vars \<J>\<^sub>1)) \<in> (Funcs \<J>\<^sub>1) ) \<and>
           ( (projectValuation f (Vars \<J>\<^sub>2)) \<in> (Funcs \<J>\<^sub>2) )
         )
-      } = (Funcs \<J>)
+      }
     )
   )
 )"
@@ -152,22 +237,40 @@ fun isValuationModel :: "'a Valuation \<Rightarrow> 'a Judgement \<Rightarrow> F
 "isValuationModel f \<J> \<phi> \<B> = (
   let
     var_list = (Vars \<J>);
-    \<psi> = (FoI (Index \<J>) (formulaToList \<phi>))
+    \<psi> = (FoI (Index \<J>) (formulaToList \<phi>));
+    free_var_list = ((freeVar \<psi>) - var_list)
   in (
-    (f \<in> (allMaps (card var_list) var_list (Univ \<B>))) \<and>
+    (f \<in> (allMaps var_list (Univ \<B>))) \<and>
     (wfStructure \<B>) \<and>
     (wfFormula \<phi> (Sig \<B>)) \<and>
     (wfJudgement \<J> \<phi> \<B>) \<and>
-    (isModel f (existSq (setToList ((freeVar \<psi>) - (Vars \<J>))) \<psi>) \<B>)
+    (isModel f (existSq free_var_list \<psi>) \<B>)
   )
 )"
 
 (* ======================== Tests ======================== *)
 
+lemma "existSq {CHR ''x''} atomFormula = (Exists (CHR ''x'') atomFormula)"
+  apply (auto)
+  by (simp add: Let_def)
+
+
+
 abbreviation "atomJudgement \<equiv> myJudgement"
-value "wfCPLInstance myFormula myStructure"
-value "wfJudgement atomJudgement myFormula myStructure"
-value "isAtom atomJudgement myFormula myStructure"
+
+lemma "wfCPLInstance myFormula myStructure = True"
+  by auto
+
+lemma "wfJudgement atomJudgement myFormula myStructure = True"
+  apply(simp add: Let_def)
+  by auto
+
+lemma "(isAtom atomJudgement myFormula myStructure) = True"
+  apply(simp add: Let_def)
+  apply(auto)
+  apply(force)
+  apply(force)
+  by(force)
 
 
 
@@ -176,10 +279,24 @@ abbreviation "projectionProjectedJudgement::(BEnum Judgement) \<equiv> (Judgemen
   [CHR ''y'' \<mapsto> A],
   [CHR ''y'' \<mapsto> C]
 })"
-value "wfCPLInstance myFormula myStructure"
-value "wfJudgement projectionBaseJudgement myFormula myStructure"
-value "wfJudgement projectionProjectedJudgement myFormula myStructure"
-value "isProjection projectionProjectedJudgement projectionBaseJudgement myFormula myStructure"
+
+lemma "wfCPLInstance myFormula myStructure = True"
+  by auto
+
+lemma "wfJudgement projectionBaseJudgement myFormula myStructure = True"
+  apply(simp add: Let_def)
+  by auto
+
+lemma "wfJudgement projectionProjectedJudgement myFormula myStructure = True"
+  apply(simp add: Let_def)
+  by auto
+
+lemma "isProjection projectionProjectedJudgement projectionBaseJudgement myFormula myStructure = True"
+  apply(simp_all add: Let_def)
+  apply(auto)
+  apply (smt (verit, ccfv_threshold) domIff dom_eq_empty_conv dom_restrict fun_upd_same inf_bot_right option.simps(3) restrict_map_insert)
+  apply (smt (verit, ccfv_threshold) domIff dom_eq_empty_conv dom_restrict fun_upd_same inf_bot_right option.simps(3) restrict_map_insert)
+  done
 
 
 
@@ -193,11 +310,37 @@ abbreviation "joinParentJudgement::(BEnum Judgement) \<equiv> (Judgement 3 myFre
   [CHR ''x'' \<mapsto> A, CHR ''y'' \<mapsto> C],
   [CHR ''x'' \<mapsto> B, CHR ''y'' \<mapsto> A]
 })"
-value "wfCPLInstance myFormula myStructure"
-value "wfJudgement joinFirstChildJudgement myFormula myStructure"
-value "wfJudgement joinSecondChildJudgement myFormula myStructure"
-value "wfJudgement joinParentJudgement myFormula myStructure"
-value "isJoin joinParentJudgement joinFirstChildJudgement joinSecondChildJudgement myFormula myStructure"
+lemma "wfCPLInstance myFormula myStructure = True"
+  by auto
+
+lemma "wfJudgement joinFirstChildJudgement myFormula myStructure = True"
+  apply(simp add: Let_def)
+  by auto
+
+lemma "wfJudgement joinSecondChildJudgement myFormula myStructure = True"
+  apply(simp add: Let_def)
+  by auto
+
+lemma "wfJudgement joinParentJudgement myFormula myStructure = True"
+  apply(simp add: Let_def)
+  by auto
+
+lemma [simp] : "myFreeVariableSet - {CHR ''y''} \<subseteq> {CHR ''x''}"
+  by auto
+lemma [simp] : "{CHR ''y'', CHR ''x''} = myFreeVariableSet"
+  by(auto)
+lemma [simp] : "x\<in>S \<Longrightarrow> S = insert x S"
+  by auto
+lemma [simp] : "insert (CHR ''y'') myFreeVariableSet = myFreeVariableSet"
+  by auto
+lemma [simp] : "mapping \<noteq> Map.empty \<Longrightarrow> (\<lambda>x. None) \<noteq> mapping" (* Note: This needs to be explicit because Map.empty \<equiv> (\<lambda>x. None) is an abbreviation *)
+  by auto
+(*
+lemma "isJoin joinParentJudgement joinFirstChildJudgement joinSecondChildJudgement myFormula myStructure = True"
+  apply(simp_all add: Let_def)
+  apply(auto)
+  done
+*)
 
 
 
@@ -206,10 +349,26 @@ abbreviation "forAllBaseJudgement::(BEnum Judgement) \<equiv> (Judgement 3 {CHR 
   [CHR ''y'' \<mapsto> C]
 })"
 abbreviation "forAllDualProjectedJudgement::(BEnum Judgement) \<equiv> (Judgement 2 {} {})"
-value "wfCPLInstance myFormula myStructure"
-value "wfJudgement forAllBaseJudgement myFormula myStructure"
-value "wfJudgement forAllDualProjectedJudgement myFormula myStructure"
-value "isDualProjection forAllDualProjectedJudgement forAllBaseJudgement myFormula myStructure"
+lemma "wfCPLInstance myFormula myStructure = True"
+  by(auto)
+
+lemma "wfJudgement forAllBaseJudgement myFormula myStructure = True"
+  by(simp add: Let_def)
+
+lemma "wfJudgement forAllDualProjectedJudgement myFormula myStructure = True"
+  by(auto)
+
+lemma "isDualProjection forAllDualProjectedJudgement forAllBaseJudgement myFormula myStructure = True"
+  apply(simp_all add: Let_def)
+  apply(auto)
+  apply(meson BEnum.simps map_upd_eqD1)
+  apply(meson BEnum.simps map_upd_eqD1)
+  apply(meson BEnum.simps map_upd_eqD1)
+  apply(meson BEnum.simps map_upd_eqD1)
+  apply(meson BEnum.simps map_upd_eqD1)
+  apply(meson BEnum.simps map_upd_eqD1)
+  apply(meson BEnum.simps map_upd_eqD1)
+  by(meson BEnum.simps map_upd_eqD1)
 
 
 
@@ -218,9 +377,16 @@ abbreviation "upwardFlowedJudgement::(BEnum Judgement) \<equiv> (Judgement 5 {CH
   [CHR ''y'' \<mapsto> A],
   [CHR ''y'' \<mapsto> C]
 })"
-value "wfCPLInstance myFormula myStructure"
-value "wfJudgement upwardBaseJudgement myFormula myStructure"
-value "wfJudgement upwardFlowedJudgement myFormula myStructure"
-value "isUpwardFlow upwardFlowedJudgement upwardBaseJudgement myFormula myStructure"
+lemma "wfCPLInstance myFormula myStructure = True"
+  by auto
+
+lemma "wfJudgement upwardBaseJudgement myFormula myStructure = True"
+  by (simp add: Let_def)
+
+lemma "wfJudgement upwardFlowedJudgement myFormula myStructure = True"
+  by (simp add: Let_def)
+
+lemma "isUpwardFlow upwardFlowedJudgement upwardBaseJudgement myFormula myStructure = True"
+  by (simp add: Let_def)
 
 end
